\documentclass[12pt]{article}%
\usepackage{amsfonts}
\usepackage{fancyhdr}
\usepackage{comment}
\usepackage[a4paper, top=2.5cm, bottom=2.5cm, left=2.2cm, right=2.2cm]%
{geometry}
\usepackage{times}
\usepackage{textcomp}
\usepackage{amsmath}
\usepackage{changepage}
\usepackage{amssymb}
\usepackage{graphicx}%
\setcounter{MaxMatrixCols}{30}
\newtheorem{theorem}{Theorem}
\newtheorem{acknowledgement}[theorem]{Acknowledgement}
\newtheorem{algorithm}[theorem]{Algorithm}
\newtheorem{axiom}{Axiom}
\newtheorem{case}[theorem]{Case}
\newtheorem{claim}[theorem]{Claim}
\newtheorem{conclusion}[theorem]{Conclusion}
\newtheorem{condition}[theorem]{Condition}
\newtheorem{conjecture}[theorem]{Conjecture}
\newtheorem{corollary}[theorem]{Corollary}
\newtheorem{criterion}[theorem]{Criterion}
\newtheorem{definition}[theorem]{Definition}
\newtheorem{example}[theorem]{Example}
\newtheorem{exercise}[theorem]{Exercise}
\newtheorem{lemma}[theorem]{Lemma}
\newtheorem{notation}[theorem]{Notation}
\newtheorem{problem}[theorem]{Problem}
\newtheorem{proposition}[theorem]{Proposition}
\newtheorem{remark}[theorem]{Remark}
\newtheorem{solution}[theorem]{Solution}
\newtheorem{summary}[theorem]{Summary}
\newenvironment{proof}[1][Proof]{\textbf{#1.} }{\ \rule{0.5em}{0.5em}}

\newcommand{\Q}{\mathbb{Q}}
\newcommand{\R}{\mathbb{R}}
\newcommand{\C}{\mathbb{C}}
\newcommand{\Z}{\mathbb{Z}}

\begin{document}

\title{ECON 21020 92 Econometrics}
\author{Xinxiang Liu}
\date{\today}
\maketitle


\section{Question 1}
a)  The variance of X is 560 and the variance of Y is 569.\par
\vspace{5mm} %5mm vertical space

\noindent b)  Proposed estimator:
\begin{eqnarray*}
t = \frac{(\bar{Y}-\bar{X})-(\mu_Y-\mu_X)}{\sqrt[]{\frac{s_Y^2}{n_Y}+\frac{s_X^2}{n_X}}
} = \frac{(569 - 560) - 0}{\sqrt[]{\frac{569}{44}+\frac{560}{46}}
} \approx 1.796
\end{eqnarray*} 
\vspace{5mm} %5mm vertical space

\noindent c) $H_0$: $\mu_Y$ - $\mu_X$ = 0 \par
\vspace{5mm} %5mm vertical space
\noindent\                        \                        \ $H_A$: $\mu_Y$ - $\mu_X$ > 0\par
\setlength{\leftskip}{0pt}
\vspace{5mm} %5mm vertical space
\noindent d) At $\alpha$ = 5\%, \[df = \frac{(\frac{s_X^2}{n_X}+\frac{s_Y^2}{n_Y})^2}{\frac{(\frac{s_X^2}{n_X})^2}{n_X-1}+\frac{(\frac{s_Y^2}{n_Y})^2}{n_Y-1}}\approx 88\]
\[t*\approx 1.66 < t-statistic\]\par
Therefore, we reject the Null hypothesis. \par
\vspace{5mm} %5mm vertical space

\noindent e) Let P(ID) = 1 - P($\bar{ID}$) = probability of spam filter identifying an email as spam; \par
\vspace{5mm} %5mm vertical space
\noindent\                        \                        \  P(S) = 1 - P($\bar{S}$) = probability of any given email being spam\par
\vspace{5mm} %5mm vertical space
\noindent\                        \                        \  We know from the problem statement that P(ID) = 2000/5000 = 0.4\par
\vspace{5mm} %5mm vertical space
\noindent\                        \                        \  From Bayes' Theorem we also know that P(S,ID) = 0.9P(ID) and \\
\[0.05=\frac{P(\bar{S},ID)}{P(\bar{S})}=\frac{(P(ID)-P(S,ID)}{(1-P(S)}=\frac{0.1P(ID)}{1-P(S)}=\frac{0.04}{1-P(S)}\]\par
\noindent\                        \                        \ Therefore, P(S) = 0.2.


\section{Question 2}
\begin{flalign*}
a)\hspace{5pt}&VAR(X-Y) = \mathbb{E}[(X-Y)^2] -\mathbb{E}[X-Y]^2 &&\\
&= \mathbb{E}[X^2-2XY+Y^2] - \mathbb{E}[X-Y]^2  &&\\
&= \mathbb{E}[X^2] - 2\mathbb{E}[XY] + \mathbb{E}[Y^2] - (\mathbb{E}[X] - \mathbb{E}[Y)]^2 &&\\
&= \mathbb{E}[X^2] - 2\mathbb{E}[XY] + \mathbb{E}[Y^2] - \mathbb{E}[X]^2 + \mathbb{E}[Y]^2 - 2\mathbb{E}[X]\mathbb{E}[Y]&&\\
&=(\mathbb{E}[X^2] - \mathbb{E}[X]^2) + (\mathbb{E}[Y^2] - \mathbb{E}[Y]^2) - 2(\mathbb{E}[XY] - \mathbb{E}[X]\mathbb{E}[Y])&&\\
&=VAR[X] + VAR[Y] - 2Cov[X,Y] &&\\
\end{flalign*}
\begin{flalign*}
b)\hspace{5pt}&\mathbb{E}[X] = \mu_X, \hspace{5pt}\mathbb{E}[Y] = \mu_Y &&\\
&\leadsto \mathbb{E}[a+bX] = a+b\mu_X,\hspace{5pt} \mathbb{E}[c+dY] = c+d\mu_Y &&\\
&\leadsto (a+bx) - \mathbb{E}[a+bX] = b(x=\mu_X),\hspace{5pt} (c+dy) - \mathbb{E}[c+dY] = d(y-\mu_Y) &&\\
\end{flalign*}
\begin{flalign*}
\hspace{26pt}\leadsto Cov(a+bX,\hspace{2pt}c+dY) &= \sum_{x}\sum_{y}[b(x-\mu_X)][d(y-\mu_Y)]p(x,y)&&\\
&= bd\sum_{x}\sum_{y}(x-\mu_X)(y-\mu_Y)p(x,y)&&\\
&=bdCov(X,Y)&&\\
\end{flalign*}
c)\hspace{5pt}Using Law of Iterated Expectations, where $\mathbb{E}[\mathbb{E}[Y|X]] = \mathbb{E}[Y]$, we can derive that $\mathbb{E}[Y] = c$.\par
\noindent\                        \                   \          \ Therefore, X and Y are mean-independent given that $\mathbb{E}[Y] = \mathbb{E}[Y|X] = c$\\
\vspace{5mm}\\d)\[Cov(X,Y) = \mathbb{E}[(X-\mu_X)(Y-\mu_Y)]\]
\[= \mathbb{E}[XY-\mu_XY-X\mu_Y+\mu_X\mu_Y]\]
\[= \mathbb{E}[XY]-\mu_X\mathbb{E}(Y)-\mathbb{E}(X)\mu_Y+\mu_X\mu_Y\]
\[=\mathbb{E}[XY]-\mu_X\mu_Y\]
\[=\mathbb{E}[X]\mathbb{E}[Y]-\mu_X\mu_Y = 0\] \\
\begin{flalign*}
e)\hspace{5pt} Let\hspace{5pt}g(x) &= \mathbb{E}[Y|X=x]&&\\
\leadsto\mathbb{E}[g(X)] &= \int_{\infty}^{-\infty} g(x)f_X(x) dx &&\\
&=\int_{\infty}^{-\infty} \mathbb{E}[Y|X=x]f_X(x) dx &&\\
&=\int_{\infty}^{-\infty}(\int_{\infty}^{-\infty} y\frac{f_X_Y(x,y)}{f_X(x)}dy)f_X(x)dx &&\\
&=\int_{\infty}^{-\infty}\int_{\infty}^{-\infty}yf_X_Y(x,y)dydx &&\\
&=\int_{\infty}^{-\infty}y(\int_{\infty}^{-\infty}f_X_Y(x,y)dx)dy &&\\
&=\int_{\infty}^{-\infty}yf_Y(y)dy=\mathbb{E}[Y] &&\\
\end{flalign*}

\section{Question 3}



\end{document}